some progress

Find.dfy
@@ -1,53 +1,109 @@
 /* Challenge 2 */
 
-method Find (A : array<int>, K : int) returns (s : int , l : int)
-  modifies A;
-  requires 1 <= K <= A.Length;
-  ensures 0 <= s < K <= l <= A.Length;
-  ensures forall i, j :: 0 <= i < s <= j < A.Length ==> A[i] < A[j];
-  ensures forall i, j :: 0 <= i < l <= j < A.Length ==> A[i] < A[j];
-  ensures forall i, j :: s <= i <= j < l ==> A[i] == A[j];
+//include "Partition.dfy"
+
+// TODO: Another predicate for well no change in arr
+
+predicate inplace(a : array<int>, l : int, m : int, u : int)
+  requires 0 <= l <= m <= u <= a.Length;
+  reads a;
 {
-  s, l := 0, A.Length; 
-  //var done := false;
-  var done := A.Length <= 1;
-  var m, n := s, l;
-  var w, X := s, A[K-1];
-  while !done
-    decreases !done;
-    decreases l-s;
-    invariant 0 <= s < K <= l <= A.Length;
-    invariant forall i, j :: 0 <= i < s <= j < A.Length ==> A[i] < A[j];
-    invariant forall i, j :: 0 <= i < l <= j < A.Length ==> A[i] < A[j];
-    invariant done ==> forall i, j :: s <= i <= j < l ==> A[i] == A[j];
+  forall i,j :: l <= i < m <= j < u ==> a[i] < a[j]
+}
+
+method Swap(a : array<int>, k : int, k' : int)
+  requires a.Length > 0;
+  requires 0 <= k < a.Length;
+  requires 0 <= k' < a.Length;
+  modifies a;
+  ensures a[k] == old(a[k']);
+  ensures a[k'] == old(a[k]);
+  ensures forall i :: 0 <= i < a.Length && i !in {k, k'} ==> a[i] == old(a[i])
+  ensures multiset(a[..]) == multiset(old(a[..]))
+{
+  a[k], a[k'] := a[k'], a[k];
+}
+
+method Partition(A : array<int>, s : int, l : int, X : int) returns (m : int, n : int)
+  requires A.Length > 0;
+  requires s <= l;
+  requires 0 <= s <= l <= A.Length;
+  requires 0 < s <= l <= A.Length ==> inplace(A, 0, s, A.Length);
+  requires 0 <= s <= l < A.Length ==> inplace(A, 0, l, A.Length);
+
+  modifies A;
+
+  /* Expected behaviour */
+  ensures 0 <= s <= m <= n <= l <= A.Length
+  ensures forall i :: s <= i < m ==> A[i] < X;
+  ensures forall i :: m <= i < n ==> A[i] == X;
+  ensures forall i :: n <= i < l ==> A[i] > X;
+  /* No unexpected changes occured */
+  ensures s > 0 ==> forall i :: 0 <= i < s ==> A[i] == old(A[i]);
+  ensures l < A.Length ==> forall i :: l <= i < A.Length ==> A[i] == old(A[i]);
+  ensures multiset(A[..]) == multiset(old(A[..]));
+  /* Assure partitioning is maintained */
+  ensures 0 < s <= l <= A.Length ==> inplace(A, 0, s, A.Length);
+  ensures 0 <= s <= l < A.Length ==> inplace(A, 0, l, A.Length);
+
+{
+  var k := s;
+  m, n := s, l;
+  while k < n
+    invariant 0 <= s <= m <= k <= n <= l <= A.Length;
+    invariant forall i :: s <= i < m ==> A[i] < X;
+    invariant forall i :: m <= i < k ==> A[i] == X;
+    invariant forall i :: n <= i < l ==> A[i] > X;
+    invariant s > 0 ==> forall i :: 0 <= i < s ==> A[i] == old(A[i]);
+    invariant l < A.Length ==> forall i :: l <= i < A.Length ==> A[i] == old(A[i]);
+    invariant 0 < s <= l <= A.Length ==> inplace(A, 0, s, A.Length);
+    invariant 0 <= s <= l < A.Length ==> inplace(A, 0, l, A.Length);
+    invariant multiset(A[..]) == multiset(old(A[..]));
+
+    decreases n - k;
   {
-    m, w, n, X := s, s, l, A[K-1];
-    while w < n
-      invariant s <= m <= w <= n <= l;
-      invariant forall i :: s <= i < m ==> A[i] < X;
-      invariant forall i :: m <= i < w ==> A[i] == X;
-      invariant forall i :: n <= i < l ==> A[i] > X;
-      invariant forall i, j :: 0 <= i < s <= j < A.Length ==> A[i] < A[j];
-      invariant forall i, j :: 0 <= i < l <= j < A.Length ==> A[i] < A[j];
-      invariant done ==> forall i, j :: s <= i <= j < l ==> A[i] == A[j];
-    {
-      if A[w] < X {
-        A[m], A[w] := A[w], A[m];
-        m, w := m + 1, w + 1;
-      } else if A[w] == X {
-        w := w + 1;
-      } else {
-        A[n-1], A[w] := A[w], A[n-1];
-        n := n - 1;
-      }
+
+    if A[k] < X {
+      Swap(A, m, k);
+      m := m + 1;
+      k := k + 1;
+    } else if A[k] == X {
+      k := k + 1;
+    } else if A[k] > X {
+      Swap(A, n-1, k);
+      n := n - 1;
     }
+  }
+}
+
+method Find(A : array<int>, K : int) returns (s : int , l : int)
+  requires A.Length > 0;
+  requires 1 <= K <= A.Length;
+  modifies A;
+  ensures 0 <= s < K <= l <= A.Length;
+  ensures forall i,j :: 0 <= i < s <= j < A.Length ==> A[i] < A[j];
+  ensures forall i,j :: 0 <= i < l <= j < A.Length ==> A[i] < A[j];
+  ensures forall i,j :: s <= i <= j < l ==> A[i] == A[j];
+  ensures A[s] == A[K-1];
+{
+  s, l := 0, A.Length;
+  var done := false;
+  while !done
+    invariant 0 <= s < K <= l <= A.Length
+    invariant forall i,j :: 0 <= i < s <= j < A.Length ==> A[i] < A[j];
+    invariant forall i,j :: 0 <= i < l <= j < A.Length ==> A[i] < A[j];
+    invariant done ==> forall i,j :: s <= i <= j < l ==> A[i] == A[j];
+
+    decreases !done, l - s;
+  {
+    var X := A[K-1];
+    var m, n := Partition(A, s, l, X);
     if n < K {
       s := n;
     } else if m < K <= n {
       s, l, done := m, n, true;
-    } else {
+    } else if K <= m {
       l := m;
     }
   }
-
 }
