Partition.dfy
@@ -1,35 +1,111 @@
 /* Challenge 1 */
 
-method Partition (A : array<int>, s : int, l : int, X : int) returns (m : int, n : int)
-  modifies A
-  requires 0 <= s <= l <= A.Length
-  /* Ensures *m* and *n* are inside the segment */
-  ensures s <= m <= n <= l
-  ensures forall i :: s <= i < m ==> A[i] < X
-  ensures forall i :: m <= i < n ==> A[i] == X
-  ensures forall i :: n <= i < l ==> A[i] > X
-  /* All the other elements should be left unchanged */
-  ensures (A[..s] == old(A[..s])) && (A[l..] == old(A[l..]))
-  ensures multiset(A[..]) == multiset(old(A[..]))
+//method Partition(A : array<int>, s : int, l : int, X : int) returns (m : int, n : int)
+//  requires 0 <= s <= l <= A.Length
+//  modifies A;
+//  /* Expected behaviour */
+//  ensures s <= m <= n <= l
+//  ensures forall i :: s <= i < m ==> A[i] < X;
+//  ensures forall i :: m <= i < n ==> A[i] == X;
+//  ensures forall i :: n <= i < l ==> A[i] > X;
+//  /* No unexpected changes occured */
+//  ensures A[..s] + A[l..] == old(A[..s] + A[l..])
+//  ensures multiset(A[..]) == multiset(old(A[..]));
+//{
+//  var w := s;
+//  m, n := s, l;
+//  while w < n
+//    invariant 0 <= s <= m <= w <= n <= l <= A.Length;
+//    invariant forall i :: s <= i < m ==> A[i] < X;
+//    invariant forall i :: m <= i < w ==> A[i] == X;
+//    invariant forall i :: n <= i < l ==> A[i] > X;
+//    invariant A[..s] + A[l..] == old(A[..s] + A[l..])
+//    invariant multiset(A[..]) == multiset(old(A[..]));
+//  {
+//
+//    if A[w] < X {
+//      // Swap A[m] with A[w]
+//      A[m], A[w] := A[w], A[m];
+//      m := m + 1;
+//      w := w + 1;
+//    } else if A[w] == X {
+//      w := w + 1;
+//    } else if A[w] > X {
+//      // Swap A[n-1] with A[w]
+//      A[n-1], A[w] := A[w], A[n-1];
+//      n := n - 1;
+//    }
+//  }
+//}
+
+predicate inplace(a : array<int>, l : int, m : int, h : int)
+  requires 0 <= l <= m <= h <= a.Length;
+  reads a;
 {
-  var w := s;
+  forall i,j :: l <= i < m <= j < h ==> a[i] < a[j]
+}
+
+method Swap(a : array<int>, k : int, k' : int)
+  requires a.Length > 0;
+  requires 0 <= k  < a.Length;
+  requires 0 <= k' < a.Length;
+  modifies a;
+  ensures a[k] == old(a[k']);
+  ensures a[k'] == old(a[k]);
+  ensures forall i :: (0 <= i < a.Length) && (i !in {k, k'}) ==> a[i] == old(a[i])
+  ensures multiset(a[..]) == multiset(old(a[..]))
+{
+  a[k], a[k'] := a[k'], a[k];
+}
+
+method Partition(A : array<int>, s : int, l : int, X : int) returns (m : int, n : int)
+  requires A.Length > 0;
+  requires 0 <= s <= l <= A.Length;
+  requires 0 <  s <= l <= A.Length ==> inplace(A, 0, s, A.Length);
+  requires 0 <= s <= l <  A.Length ==> inplace(A, 0, l, A.Length);
+
+  modifies A;
+
+  /* Expected behaviour */
+  ensures 0 <= s <= m <= n <= l <= A.Length
+  ensures forall i :: s <= i < m ==> A[i] < X;
+  ensures forall i :: m <= i < n ==> A[i] == X;
+  ensures forall i :: n <= i < l ==> A[i] > X;
+  /* No unexpected changes occured */
+  ensures s > 0        ==> forall i :: 0 <= i < s        ==> A[i] == old(A[i]);
+  ensures l < A.Length ==> forall i :: l <= i < A.Length ==> A[i] == old(A[i]);
+  ensures multiset(A[..]) == multiset(old(A[..]));
+  /* Assure partitioning is maintained */
+  ensures 0 <  s <= l <= A.Length ==> inplace(A, 0, s, A.Length);
+  ensures 0 <= s <= l <  A.Length ==> inplace(A, 0, l, A.Length);
+
+{
+  var k := s;
   m, n := s, l;
-  while w < n
-    invariant s <= m <= w <= n <= l
-    invariant forall i :: s <= i < m ==> A[i] < X
-    invariant forall i :: m <= i < w ==> A[i] == X
-    invariant forall i :: n <= i < l ==> A[i] > X
-    invariant forall i :: 0 <= i < s ==> A[i] == old(A[i])
-    invariant forall i :: l <= i < A.Length ==> A[i] == old(A[i])
-    invariant multiset(A[..]) == multiset(old(A[..]))
+  while k < n
+    invariant 0 <= s <= m <= k <= n <= l <= A.Length;
+    invariant forall i :: s <= i < m ==> A[i] < X;
+    invariant forall i :: m <= i < k ==> A[i] == X;
+    invariant forall i :: n <= i < l ==> A[i] > X;
+    /* No unexpected changes occured */
+    invariant s > 0        ==> forall i :: 0 <= i < s        ==> A[i] == old(A[i]);
+    invariant l < A.Length ==> forall i :: l <= i < A.Length ==> A[i] == old(A[i]);
+    invariant multiset(A[..]) == multiset(old(A[..]));
+    /* Assure partitioning is maintained */
+    invariant 0 < s <= l <= A.Length ==> inplace(A, 0, s, A.Length);
+    invariant 0 <= s <= l < A.Length ==> inplace(A, 0, l, A.Length);
+
+    decreases n - k;
   {
-    if A[w] < X {
-      A[m], A[w] := A[w], A[m];
-      m, w := m + 1, w + 1;
-    } else if A[w] == X {
-      w := w + 1;
-    } else {
-      A[n-1], A[w] := A[w], A[n-1];
+
+    if A[k] < X {
+      Swap(A, m, k);
+      m := m + 1;
+      k := k + 1;
+    } else if A[k] == X {
+      k := k + 1;
+    } else if A[k] > X {
+      Swap(A, n-1, k);
       n := n - 1;
     }
   }
